arm/ed25519/code/ed25519_s2n_bignum.h
@@ -5,7 +5,7 @@
 #define ED25519_SIGNATURE_LEN 64
 #define ED25519_PRIVATE_KEY_LEN 64
 
-void ed25519_keypair_from_seed_s2n_bignum (
+void ed25519_public_key_from_seed_s2n_bignum (
 						uint8_t A[ED25519_PUBLIC_KEY_LEN],
 						const uint8_t seed[ED25519_SEED_LEN]);
 
